HelloTypeSystem/Meta/ML3/Typing.lean
@@ -1,0 +1,98 @@
+import HelloTypeSystem.ML3
+
+namespace HelloTypeSystem.ML3
+open ML3
+
+/-!
+# ML3に対する型付け
+-/
+
+/-
+## TypingML3における型判断の導出例
+
+### 練習問題8.1
+-/
+
+example : Typed [("y", .Int), ⟨"x", .Bool⟩] (.If "x" ("y" + 1) ("y" - 1)) .Int :=
+  (.If
+    (.VarIr .Var)
+    (.Add .Var .Int)
+    (.Sub .Var .Int)
+  )
+
+example : Typed [] (.Let "x" (.LT 3 2) (.Let "y" 5 (.If "x" "y" 2))) .Int :=
+  -- let x = (3 : Int) < (2 : Int) : Bool in
+  (.Let
+    (.LT .Int .Int)
+    -- let y = 5 : Int in
+    (.Let
+      (.Int)
+      (.If (.VarIr .Var) (.Var) (.Int))
+    )
+  )
+
+example : Typed [] (.Fn "x" ("x" + 1)) (.Fn .Int .Int) :=
+  (.Fn (.Add .Var .Int))
+
+example : Typed [] (.Fn "f" ((.App "f" 0) + (.App "f" 1))) (.Fn (.Fn .Int .Int) .Int) :=
+  (.Fn
+    (.Add
+      (.App .Var .Int)
+      (.App .Var .Int)
+    )
+  )
+
+example : Typed [] (.Let "k" (.Fn "x" (.Fn "y" "x")) (.App (.App "k" 3) true)) .Int :=
+  (.Let
+    (.Fn (.Fn (.VarIr .Var)))
+    (.App
+      (.App .Var .Int)
+      (.Bool)
+    )
+  )
+
+example : Typed []
+  (
+    (.Let "compose"
+      /- := -/
+      (.Fn "f"
+        (.Fn "g"
+          (.Fn "x"
+            (.App "f" (.App "g" "x"))
+          )
+        )
+      )
+      /- in -/
+      (.Let "p" (.Fn "x" ("x" * "x"))
+        /- in -/
+        (.Let "q" (.Fn "x" ("x" + 4))
+          /- in -/
+          (.App (.App "compose" "p") "q") -- compose p q
+        )
+      )
+    )
+  )
+  (.Fn .Int .Int)
+:=
+  (.Let
+    (.Fn
+      (.Fn
+        (.Fn
+          (.App
+            (.VarIr (.VarIr .Var))
+            (.App (.VarIr .Var) .Var)
+          )
+        )
+      )
+    )
+    (.Let
+      (.Fn (.Mul .Var .Var))
+      (.Let
+        (.Fn (.Add .Var .Int))
+        (.App
+          (.App (.VarIr (.VarIr .Var)) (.VarIr .Var))
+          (.Var)
+        )
+      )
+    )
+  )
